ECCA/typing.v
@@ -70,24 +70,24 @@ Inductive Types: env -> exp -> exp -> Prop :=
   (g ⊢ A : (eUni (uType i))) ->
   (Types (g & x ~ Assum A) (open x B) (eUni (uType i))) ->
   (g ⊢ (ePi A B) : (eUni (uType i)))
-| aT_Lam (g: env) (x: name) (A e B U: exp) :
-  (g ⊢ A: U) ->
+| aT_Lam (g: env) (x: name) (A e B: exp) i :
+  (g ⊢ A: eUni (uType i)) ->
   (Types (g & x ~ Assum A) (open x e) (open x B)) ->
   (g ⊢ (eAbs A e) : (ePi A B))
-| aT_Let (g: env) (n m A B U: exp) (x: name):
-  (g ⊢ A: U) ->
+| aT_Let (g: env) (n m A B: exp) (U: universe) (x: name):
+  (g ⊢ A: eUni U) ->
   (g ⊢ n : A) ->
   (Types (g & x ~ Def n A) (open x m) (open x B)) ->
   (g ⊢ (eLet n m) : (bind n B))
-| aT_If (g: env) (B U e1 e2: exp) (e: exp) (x p: name):
-  ((g & x ~ Assum eBool) ⊢ (open x B): U) -> 
+| aT_If (g: env) (B e1 e2: exp) (e: exp) (U: universe) (x p: name):
+  ((g & x ~ Assum eBool) ⊢ (open x B): eUni U) -> 
   (g ⊢ e : eBool) ->
   ((g & p ~ (Assum (eEqv e eTru))) ⊢ [^p] e1 : (bind eTru ([^p] B))) ->
   ((g & p ~ (Assum (eEqv e eFls))) ⊢ [^p] e2 : (bind eFls ([^p] B))) -> 
   (g ⊢ (eIf e e1 e2) : (bind e B)) 
-| aT_Conv (g: env) (e A B U: exp) :
+| aT_Conv (g: env) (e A B: exp) (U: universe) :
   (g ⊢ e : A) ->
-  (g ⊢ B : U) ->
+  (g ⊢ B : eUni U) ->
   (SubTypes g A B) ->
   (g ⊢ e : B)
 | aT_App (g: env) (e e': exp) (A' B: exp) :
@@ -113,13 +113,13 @@ with (* ECCA Well-Formed Environments *)
 WellFormed: env -> Prop :=
   | wf_Empty : 
     (⊢ ctx_empty)
-  | wf_Assum : forall (g : env) (x : name) (A U : exp),
+  | wf_Assum : forall (g : env) (x : name) (A: exp) (U: universe),
     (⊢ g) -> 
-    (g ⊢ A : U) -> 
+    (g ⊢ A : eUni U) -> 
     (⊢ g & x ~ Assum A)
-  | wf_Def : forall (g : env) (x : name) (e A U : exp),
+  | wf_Def : forall (g : env) (x : name) (e A: exp) (U: universe),
     (⊢ g) -> 
-    (g ⊢ A : U) -> 
+    (g ⊢ A : eUni U) -> 
     (g ⊢ e : A) -> 
     (⊢ g & x ~ Def e A)
 where "'⊢' g" := (WellFormed g) : ECCA_scope.
