ECCA/typing_lemmas.v
@@ -48,42 +48,42 @@ all: try (intros; constructor; eauto; fail).
       * apply f in H0. left. names in H0. apply H0.
       * destruct H0. apply f in H0. right. eauto. 
 + intros. names. apply aT_Sig with (x:=x). eauto.
-  names. apply IHpT2 with (Δ:= (Δ & x ~ Assum ([r] A0))) (r:= (r,, x)%ren).
-  apply ctx_rename; eauto. apply wf_Assum with (eUni (uType i)); eauto.
-+  intros. names. apply aT_Pair with ([r] U).
+  names. apply IHpT2 with (Δ:= (Δ & x ~ Assum ([r] A))) (r:= (r,, x)%ren).
+  apply ctx_rename; eauto. apply wf_Assum with (uType i); eauto.
++  intros. names. apply aT_Pair.
   - auto.
   - specialize IHpT2 with (r:=r) (Δ:=Δ). names in IHpT2. apply IHpT2; eauto.
-  - specialize IHpT3 with (r:=r) (Δ:=Δ). names in IHpT3. apply IHpT3; eauto.
+(*   - specialize IHpT3 with (r:=r) (Δ:=Δ). names in IHpT3. apply IHpT3; eauto. *)
 +  intros. names. eapply aT_Prod_Prop with (x:=x). eauto.
-  names. apply IHpT2 with (Δ:= (Δ & x ~ Assum ([r] A0))) (r:= (r,, x)%ren).
+  names. apply IHpT2 with (Δ:= (Δ & x ~ Assum ([r] A))) (r:= (r,, x)%ren).
   apply ctx_rename. auto. eauto.
 +  intros. names. eapply aT_Prod_Type with (x:=x). eauto.
-  names. apply IHpT2 with (Δ:= (Δ & x ~ Assum ([r] A0))) (r:= (r,, x)%ren).
+  names. apply IHpT2 with (Δ:= (Δ & x ~ Assum ([r] A))) (r:= (r,, x)%ren).
   apply ctx_rename. auto. eauto.
 +  intros. names. eapply aT_Lam with (x:=x). eauto.
-  names. apply IHpT2 with (Δ:= (Δ & x ~ Assum ([r] A0))) (r:= (r,, x)%ren).
-  apply ctx_rename. auto. apply wf_Assum with ([r] U); eauto.
-+  intros. names. apply aT_Let with (x:=x) (A:=([r]A0)) (U:=([r]U)); eauto.
-  names. apply IHpT3 with (Δ:= (Δ & x ~ Def ([r] n) ([r] A0))) (r:= (r,, x)%ren).
-  apply ctx_rename. auto. apply wf_Def with ([r] U); eauto.
-+  intros. names. apply aT_If with (x:=x) (p:=p) (U:=[r,,x]U). 
+  names. apply IHpT2 with (Δ:= (Δ & x ~ Assum ([r] A))) (r:= (r,, x)%ren).
+  apply ctx_rename. auto. apply wf_Assum with (uType i); eauto.
++  intros. names. apply aT_Let with (x:=x) (A:=([r]A)) (U:=U); eauto.
+  names. apply IHpT3 with (Δ:= (Δ & x ~ Def ([r] n) ([r] A))) (r:= (r,, x)%ren).
+  apply ctx_rename. auto. apply wf_Def with U; eauto.
++  intros. names. apply aT_If with (x:=x) (p:=p) (U:=U). 
   - names. apply IHpT1 with (Δ:= (Δ & x ~ Assum eBool)) (r:= (r,, x)%ren).
     apply ctx_rename. auto. eauto.
   - eauto.
   - names. specialize IHpT3 with (Δ:= (Δ & p ~ Assum (eEqv ([r] e) eTru))) (r:= (r,, p)%ren). names in IHpT3. apply IHpT3.
-    apply ctx_rename. auto. eapply wf_Assum with (eUni (uType 0)). auto.
+    apply ctx_rename. auto. eapply wf_Assum with (uType 0). auto.
     apply aT_Equiv with (B:= eBool); eauto.
   - names. specialize IHpT4 with (Δ:= (Δ & p ~ Assum (eEqv ([r] e) eFls))) (r:= (r,, p)%ren). names in IHpT4. apply IHpT4.
-    apply ctx_rename. auto. eapply wf_Assum with (eUni (uType 0)). auto.
+    apply ctx_rename. auto. eapply wf_Assum with (uType 0). auto.
     apply aT_Equiv with (B:= eBool); eauto.
-+ intros. apply aT_Conv with (A:=[r]A0)(U:=[r]U); eauto.
++ intros. apply aT_Conv with (A:=[r]A)(U:=U); eauto.
   apply SubTypes_weakening with g; auto.
 +  intros. names. apply aT_App with ([r]A').
   - apply IHpT1; auto.
   - apply IHpT2; auto.
 + intros. names. apply aT_Fst with ([r]B). apply IHpT; auto.
-+ intros. names. apply aT_Snd with ([r]A0). apply IHpT; auto.
-+ intros. names. apply aT_Refl with ([r]A0). auto.
++ intros. names. apply aT_Snd with ([r]A). apply IHpT; auto.
++ intros. names. apply aT_Refl with ([r]A). auto.
 + intros. names. apply aT_Equiv with (B:=[r]B); eauto.
 Qed.
 
@@ -95,23 +95,23 @@ all: try (intros; constructor; eauto; fail); unfold Type_weakening. *)
 
 Lemma cons_weakening_assum (g: env) (A A': exp) (x: name):
 (g ⊢ A : A') ->
-  (forall B B', 
-   ((g ⊢ B : B') -> 
+  (forall B (U: universe), 
+   ((g ⊢ B : eUni U) -> 
    (g & x ~ Assum B ⊢ [^x] A : [^x] A'))).
 Proof.
 intros. apply Type_weakening with g; auto. apply ctx_shift; apply ctx_id.
-apply wf_Assum with B'; auto. apply Types_only_if_wellformed with A A'; auto. 
+apply wf_Assum with U; auto. apply Types_only_if_wellformed with A A'; auto. 
 Qed.
 
 Lemma cons_weakening_def (g: env) (A A': exp) (x: name):
 (g ⊢ A : A') ->
-  (forall B B' e, 
-   ((g ⊢ B : B') ->
+  (forall B U e, 
+   ((g ⊢ B : eUni U) ->
     (g ⊢ e : B) ->
    (g & x ~ Def e B ⊢ [^x] A : [^x] A'))).
 Proof.
 intros. apply Type_weakening with g; auto. apply ctx_shift; apply ctx_id.
-apply wf_Def with B'; auto. apply Types_only_if_wellformed with A A'; auto.
+apply wf_Def with U; auto. apply Types_only_if_wellformed with A A'; auto.
 Qed.
 
 Require Import String.
@@ -168,12 +168,16 @@ eapply aT_Conv.
 Qed. *)
 (* Conclusion: We need to shift the bodies of ass/defs in the context when we add a new ass/def *)
 
+Lemma shift_uni_id:
+forall x U {V},
+([^x] (@eUni V U)) = (@eUni V U).
+Proof. auto. Qed.
 
 Lemma WellFormed_implies_well_typed_assum (g: env):
 WellFormed g ->
 forall (v: var) (A: exp),
 (has g v (Assum A)) ->
-exists U, Types g A U.
+exists U, Types g A (eUni U).
 Proof.
 induction 1.
 + intros. inversion H.
@@ -183,13 +187,13 @@ induction 1.
   destruct H2.
   * destruct H0 as [g']. destruct H0 as [c]. destruct H0.
     inversion H0. subst. names in H2. inversion H2. subst. destruct H0.
-    exists ([^x0] U). apply cons_weakening_assum with U; auto.
+    exists U. rewrite <- shift_uni_id with (x:=x0). apply cons_weakening_assum with U; auto.
   * destruct H0 as [g']. destruct H0. destruct H0 as [c]. destruct H0. destruct H0 as [c'].
     destruct H0. destruct H2. destruct H3. inversion H0. subst. clear H0.
     destruct H4. cut (has g' x2 c'). intro. cut (exists B, c' = Assum B). intro. 
     destruct H5 as [B]. subst. names in H3. inversion H3. subst.
-    apply IHWellFormed in H4. destruct H4 as [B']. 
-    apply cons_weakening_assum with (A:=B) (A':=B')(x:=x1) in H1.
+    apply IHWellFormed in H4. destruct H4 as [B'].
+    apply cons_weakening_assum with (A:=B) (A':=eUni B')(x:=x1) in H1.
     eauto. eauto. unfold apply in H3. destruct c'. eauto. discriminate.
     unfold has. rewrite H0. auto.
 + intros. apply has_inversion in H2. apply get_inversion in H2.
@@ -202,7 +206,7 @@ induction 1.
     cut (has g' x2 c'). cut (exists B, c' = Assum B). intros.
     destruct H2 as [B]. subst. names in H6. inversion H6. subst.
     apply IHWellFormed in H3. destruct H3 as [B'].
-    apply cons_weakening_def with (A:=B) (A':=B') (B':=U)(x:=x1) in H1.
+    apply cons_weakening_def with (A:=B) (A':=eUni B') (U:=U)(x:=x1) in H1.
     all: eauto. unfold apply in H6. destruct c'. eauto. discriminate. unfold has. rewrite H5. auto.
 Qed.
 
@@ -210,7 +214,7 @@ Lemma WellFormed_implies_well_typed_def (g: env):
 WellFormed g ->
 forall (v: var) (A: exp) (e: exp),
 (has g v (Def e A)) ->
-exists U, Types g A U.
+exists U, Types g A (eUni U).
 Proof.
 induction 1.
 + intros. inversion H.
@@ -223,36 +227,300 @@ induction 1.
     destruct H0. destruct H2. destruct H3. inversion H0. subst. clear H0.
     destruct H4. cut (has g' x2 c'). intro. cut (exists e' B, c' = Def e' B). intro. 
     destruct H5 as [e']. destruct H5 as [B]. subst. names in H3. inversion H3. subst.
-    apply IHWellFormed in H4. destruct H4 as [B']. 
-    apply cons_weakening_assum with (A:=B) (A':=B')(x:=x1) in H1.
+    apply IHWellFormed in H4. destruct H4 as [B'].
+    apply cons_weakening_assum with (A:=B) (A':=eUni B')(x:=x1) in H1.
     eauto. eauto. unfold apply in H3. destruct c'. discriminate. eauto.
     unfold has. rewrite H0. auto.
 + intros. apply has_inversion in H2. apply get_inversion in H2.
   destruct H2. destruct H2. destruct H3.
   * destruct H3 as [g']. destruct H3 as [c]. destruct H3.
     inversion H3. subst. names in H4. inversion H4. subst. destruct H4.
-    exists ([^x0] U). apply cons_weakening_def with U; auto.
+    exists U. rewrite <- shift_uni_id with (x:=x0). apply cons_weakening_def with U; auto.
   * destruct H3 as [g']. destruct H3. destruct H3 as [c]. destruct H3. destruct H3 as [c'].
     destruct H3. destruct H4. destruct H5. inversion H3. subst. clear H3.
     cut (has g' x2 c'). intro. cut (exists e' B, c' = Def e' B). intro. 
     destruct H3 as [e']. destruct H3 as [B]. subst. names in H6. inversion H6. subst.
-    apply IHWellFormed in H2. destruct H2 as [B']. exists ([^x1] B').
-    apply cons_weakening_def with (A:=B) (A':=B')(x:=x1) (B':=U); eauto.
+    apply IHWellFormed in H2. destruct H2 as [B']. exists (B').
+    apply cons_weakening_def with (A:=B) (A':=eUni B')(x:=x1) (U:=U); eauto.
     unfold apply in H6. destruct c'. discriminate. eauto.
     unfold has. rewrite H5. auto.
 Qed.
 
-Lemma type_well_typed (g: env) (N: exp) (A: exp) :
+Lemma universe_lt_st:
+forall g,
+(⊢ g) ->
+forall i i',
+(lt i i') ->
+(g ⊢ (eUni (uType i)) ≲ (eUni (uType i'))).
+Proof. 
+intros. induction H0. apply ST_Cum.
+eapply ST_Trans. apply IHle. apply ST_Cum.
+Qed.
+
+Lemma universe_lt:
+forall g,
+(⊢ g) ->
+forall i i',
+(lt i i') ->
+(g ⊢ (eUni (uType i)) : (eUni (uType i'))).
+Proof. 
+intros. induction H0.
+  - eauto.
+  - eapply aT_Conv. apply IHle. auto. auto.
+Qed.  
+
+Import Coq.Arith.Compare_dec.
+Import Lia.
+
+Lemma unis_dont_step:
+forall g U U',
+(g ⊢ eUni U ⊳ eUni U') -> U = U'.
+Proof.
+inversion 1. Qed.
+
+Lemma unis_dont_reduce:
+forall g U e,
+(g ⊢ eUni U ⊳* e) -> e = eUni U.
+Proof.
+intros. remember (eUni U) as e1 in H. 
+induction H; try discriminate.
++ subst. inversion H.
++ subst. auto.
++ subst. destruct IHReduces1. auto. apply IHReduces2. auto. 
+Qed.
+
+Lemma type_not_subtype_prop:
+forall g,
+(⊢ g) ->
+forall i,
+(g ⊢ eUni (uType i) ≲ eUni uProp) -> False.
+Proof.
+intros.
+inversion H0.
++ subst. inversion H1. subst. 
+- apply unis_dont_step in H2. discriminate.
+- subst. (* H2 : assumes g x (eEqv (eUni (uType i)) (eUni uProp))*) 
+(* there is actually nothing to prevent us from assuming things that aren't true *)
+Abort.
+
+Lemma universe_type_if:
+forall g,
+forall U e,
+(g ⊢ eUni U : e) ->
+(g ⊢ eUni U ≲ e).
+Proof. intros. remember (eUni U) as e1 in H. 
+induction H; try discriminate.
+  - inversion Heqe1. eauto.
+  - inversion Heqe1. eauto.
+  - subst. apply ST_Trans with (A':=A). apply IHTypes1. auto. auto.
+Qed.
+
+Lemma universe_type_common_parent:
+forall g,
+(⊢ g) ->
+forall i i', 
+exists i'', 
+(g ⊢ (eUni (uType i)) : (eUni (uType i''))) /\
+(g ⊢ (eUni (uType i')) : (eUni (uType i''))).
+Proof.
+intros. destruct (Nat.compare i i') eqn:Heq.
++ apply nat_compare_eq in Heq. rewrite Heq. exists (S (i')). eauto.
++ apply nat_compare_lt in Heq. exists (S i'). split.
+  apply universe_lt; eauto. eauto.
++ apply nat_compare_gt in Heq. exists (S i). split.
+  - apply universe_lt; eauto.
+  - cut (i' < i). intro. apply universe_lt; eauto. auto.
+Qed.
+
+Lemma universe_type_common_subtype:
+forall g,
+(⊢ g) ->
+forall i i', 
+exists i'', 
+(g ⊢ (eUni (uType i)) ≲ (eUni (uType i''))) /\
+(g ⊢ (eUni (uType i')) ≲ (eUni (uType i''))).
+Proof.
+intros. destruct (Nat.compare i i') eqn:Heq.
++ apply nat_compare_eq in Heq. rewrite Heq. exists (S (i')). eauto.
++ apply nat_compare_lt in Heq. exists (S i'). split.
+  apply universe_lt_st; eauto. eauto.
++ apply nat_compare_gt in Heq. exists (S i). split.
+  - apply universe_lt_st; eauto.
+  - cut (i' < i). intro. apply universe_lt_st; eauto. auto.
+Qed.
+
+Lemma universe_common_parent:
+forall g,
+(⊢ g) ->
+forall U U', 
+exists U'', 
+(g ⊢ (eUni U) : (eUni U'')) /\
+(g ⊢ (eUni U') : (eUni U'')).
+Proof.
+intros. destruct U; destruct U'.
++ exists (uType 0). auto.
++ exists (uType (S i)). split. 
+  - eapply aT_Conv. apply aT_Ax_Prop. auto. auto. apply universe_lt_st. auto. lia.
+  - apply universe_lt; auto.
++ exists (uType (S i)). split. 
+  - apply universe_lt; auto.
+  - eapply aT_Conv. apply aT_Ax_Prop. auto. auto. apply universe_lt_st. auto. lia.
++ cut (exists i'', (g ⊢ eUni (uType i) : eUni (uType i'')) /\
+  (g ⊢ eUni (uType i0) : eUni (uType i''))). intro. destruct H0. exists (uType x). auto.
+  apply universe_type_common_parent. auto.
+Qed.
+
+Lemma universe_common_parent_type:
+forall g,
+(⊢ g) ->
+forall U U', 
+exists i, 
+(g ⊢ (eUni U) : (eUni (uType i))) /\
+(g ⊢ (eUni U') : (eUni (uType i))).
+Proof.
+intros. destruct U; destruct U'.
++ eauto.
++ exists ((S i)). split. 
+  - eapply aT_Conv. apply aT_Ax_Prop. auto. auto. apply universe_lt_st. auto. lia.
+  - apply universe_lt; auto.
++ exists ((S i)). split. 
+  - apply universe_lt; auto.
+  - eapply aT_Conv. apply aT_Ax_Prop. auto. auto. apply universe_lt_st. auto. lia.
++ cut (exists i'', (g ⊢ eUni (uType i) : eUni (uType i'')) /\
+  (g ⊢ eUni (uType i0) : eUni (uType i''))). intro. destruct H0. exists (x). auto.
+  apply universe_type_common_parent. auto.
+Qed.
+
+Lemma universe_common_parent_subtype:
+forall g,
+(⊢ g) ->
+forall U U', 
+exists i, 
+(g ⊢ (eUni U) ≲ (eUni (uType i))) /\
+(g ⊢ (eUni U') ≲ (eUni (uType i))).
+Proof.
+intros. destruct U; destruct U'.
++ eauto.
++ exists ((S i)). split. 
+  - eapply ST_Trans. eapply ST_Prop. eapply universe_lt_st; auto. lia.
+  - apply universe_lt_st; auto.
++ exists ((S i)). split. 
+  - apply universe_lt_st; auto.
+  - eapply ST_Trans. eapply ST_Prop. eapply universe_lt_st; auto. lia.
++ cut (exists i'', (g ⊢ eUni (uType i) : eUni (uType i'')) /\
+  (g ⊢ eUni (uType i0) : eUni (uType i''))). intro. destruct H0. 
+  apply universe_type_common_subtype. auto. apply universe_type_common_parent. auto.
+Qed.
+
+Compute (close "x" (eId (free "x"))).
+Compute (eId (@bound 1 l0)).
+
+(*Lemma bind_inversion (a: @exp 0) (v: @exp 0) (b: @exp 1):
+bind v b = a ->
+wk a = b \/ 
+((b = (eId (@bound (1) l0))) /\ a = v)
+\/
+(exists l: level, (b = (eId (bound (S l)))) /\ a = (eId (bound l))).
+
+Proof. intros. destruct b.
++ destruct x.
+  - names in H. left. cut (@eId 1 (@free 1 name) = wk (@eId 0 (@free 0 name))).
+    * intro. rewrite H0. apply f_equal. auto.
+    * names. auto.
+  - destruct l.
+    * right. auto.
+    * left. names in H. subst. auto. 
++ names in H. left. subst. auto.
++ names in H. left. subst. auto.  *)
+
+(* Lemma substitution_definition:
+forall g v A B U, 
+(g ⊢ bind v B : eUni U) ->
+(g ⊢ v : A) ->
+forall g' r,
+relates g r g' ->
+forall x,
+has g' (free x) (Def v A) ->
+(g' ⊢ open x ([r] B): eUni U).
+Proof. intros. induction H.
++ subst.
+ *)
+
+(* I need an induction principle for V=1, not just V=0 *)
+Lemma substitution_definition:
+forall g v A B U U', 
+(g ⊢ bind v B : eUni U) ->
+(g ⊢ v : A) ->
+(g ⊢ A : eUni U') ->
+forall x, exists A', ((g & x ~ Def v A') ⊢ open x B: eUni U).
+Proof. intros. destruct B.
++ names in H. destruct x0.
+  ++ names in H. names.
+    cut ((@eId 0 (@free 0 (shift_name x name))) = ([^x] @eId 0 (@free 0 name))).
+    - intros. rewrite H2. rewrite <- shift_uni_id with (x:=x).
+      exists A. eapply cons_weakening_def. auto. eauto. auto.
+    - names. auto.
+  ++ destruct l.
+    - names. names in H. exists (eUni U). apply aT_Var. 
+      apply Types_only_if_wellformed in H0 as H2. 
+      pose universe_common_parent. destruct e with (U:=U) (U':=U) (g:=g).
+      auto. destruct H3. eapply wf_Def. auto. apply H3. 
+      apply H.
+      unfold assumes. right. exists ([^x] v).
+      apply ctx_has.
+    - names. names in H. exists A. 
+    cut (eId (bound s) = ([^x] eId (bound s))); auto.
+     * intros. simpl (0 + 0) in H2. rewrite H2.
+       rewrite <- shift_uni_id with (x:=x).
+       eapply cons_weakening_def.
+       auto. apply H1. apply H0.
++ exists A. names. names in H.
+ rewrite <- (shift_uni_id x U). 
+ rewrite <- shift_uni_id with (x:=x).
+    Check cons_weakening_def. 
+    apply cons_weakening_def with U'; auto.
++ names. names in H.
+
+
+Lemma substitution_assumption:
+forall g v A B U, 
+(g ⊢ v : A) ->
+(g ⊢ bind v B : eUni U) ->
+forall x, ((g & x ~ Assum A) ⊢ open x B: eUni U).
+Proof. intros. inversion H0.
++ subst.
+  
+
+Lemma assumption_substitution:
+forall g v A B U, 
+(g ⊢ v : A) ->
+forall x, ((g & x ~ Assum A) ⊢ open x B: eUni U) ->
+(g ⊢ bind v B : eUni U).
+Proof. Admitted.
+
+Lemma Type_well_typed (g: env) (N: exp) (A: exp) :
   (g ⊢ N : A) ->
-  exists U , Types g A (eUni (uType i)).
+  exists U , Types g A (eUni U).
 Proof.
   induction 1; eauto.
   - intros. destruct H0.
     + apply WellFormed_implies_well_typed_assum with (v:=x); auto.
     + destruct H0 as [e]. apply WellFormed_implies_well_typed_def with (v:=x) (e:=e); auto.
-  -  
-  
-  Admitted. (*  apply WellFormed_implies. intros. induction H0.
+  - destruct IHTypes1, IHTypes2. cut (exists i, (g ⊢ (eUni x): (eUni (uType i))) /\ (g ⊢ (eUni x0): (eUni (uType i)))).
+    + intro. destruct H3. exists (uType x1). apply aT_Sig with (x:="sigx").
+      * eapply aT_Conv. eauto. eauto. destruct H3. apply universe_type_if. auto.
+      * destruct H3. Check cons_weakening_assum. cut (g & "sigx" ~ Assum A ⊢ eUni x0 : eUni (uType x1)). 
+        -- intro. apply substitution_assumption with (v:=v1). auto. 
+            eapply aT_Conv. eauto. eauto. apply universe_type_if. auto.
+        -- Check cons_weakening_assum. apply cons_weakening_assum with (B:=A) (U:=x) (A:=eUni x0) (A':=eUni (uType x1)) (x:="sigx"). auto. auto. 
+    + apply universe_common_parent_type. eauto.
+  - destruct IHTypes1. destruct IHTypes2. destruct x1.
+    + exists uProp. eapply aT_Prod_Prop. eauto. eauto.
+    + pose universe_common_parent_type. specialize e0 with (U:=uType i) (U':=uType i0) (g:=g). destruct e0. eauto. destruct H3.
+      exists (uType x1). eapply aT_Prod_Type with (x:=x).
+        * eapply aT_Conv. eauto. eauto. apply universe_type_if. auto.
+        * eapply cons_weakening_assum with (B:=A) (x:=x) in H4. names in H4. eapply aT_Conv; eauto. apply universe_type_if. auto. eauto.
+  -  Admitted. (*  apply WellFormed_implies. intros. induction H0.
     + subst. destruct H; destruct h. 
     + subst. destruct H. cbn in h. destruct (bindv (closev x0 x)).
       * names.  
@@ -277,6 +545,71 @@ Lemma has_type_wf_g (g: env) (N: exp) (A: exp) (x : name):
   WellFormed g ->
   WellFormed (g & x ~ (Def N A)).
 Proof.
-  intros.  apply type_well_typed in H as H1; auto. destruct H1.
+  intros.  apply Type_well_typed in H as H1; auto. destruct H1.
   apply wf_Def with (U := x0); auto.
-Qed.  *)
+Qed.
+
+Lemma append_env_weakening (g g': env):
+  exists r, relates g' r (core.append g g').
+Proof.
+induction g.
++ exists r_id. cbn. apply ctx_id.
++ cbn. destruct IHg as [r]. exists (r,,^a)%ren. apply ctx_shift. auto.
+Qed.
+
+Lemma append_env_equiv_weakening (g g': env) (e e' : exp):
+  Equiv g e e' ->
+  Equiv (core.append g g') e e'.
+Proof.
+Admitted.
+
+(*
+Lemma append_env_weakening (g g': env) (N A : exp):
+  Types g N A ->
+  Types (core.append g g') N A.
+Proof.
+intros. 
+
+Lemma append_env_equiv_weakening (g g': env) (e e' : exp):
+  Equiv g e e' ->
+  Equiv (append g g') e e'.
+Proof.
+Admitted. *)
+
+Definition gbad:=
+(ctx_empty & "e" ~ (Assum (eEqv eTru eFls))
+& "P" ~ (Assum (ePi eBool (eUni (uType 0))))
+& "f" ~ (Assum (ePi (eApp (eId (free "P")) eTru) eBool))
+& "x" ~ (Assum (eApp (eId (free "P")) eFls))).
+
+Lemma gbad_wf: WellFormed gbad. Admitted.
+
+Lemma bad2:
+forall g ->
+WellFormed g ->
+forall e P f x, 
+Types g e (eEqv eTru eFls) ->
+Types g P 
+
+Lemma bad1: 
+let expr:=(@eAbs 0 (eEqv eTru eFls) (eApp ((eId (free "f"))) (eId (free "x"))))
+in 
+(Types gbad
+(eApp expr (eId (free "e"))) (bind expr eBool)).
+Proof. intros. unfold expr. apply aT_App with (A' := (eEqv eTru eFls)). 
++ apply aT_Lam with (x:="z") (i:=0).
+  - apply aT_Equiv with (B:=eBool).
+    * apply aT_True. apply gbad_wf.
+    * apply aT_False. apply gbad_wf.
+    * apply aT_Bool. apply gbad_wf.
+  - 
+
+
+(* /\
+(Reduces (ctx_empty & e ~ (Assum (eEqv eTru eFls))
+& P ~ (Assum (ePi eBool (eUni (uType 0))))
+& f ~ (ePi (eApp P eTru) eBool
+& x ~ (P eFls))) (eApp (eAbs (eEqv t u) (f x)) e) (f e)).
+ *)
+
+
