ECCA/continuations_lemmas.v
@@ -94,12 +94,16 @@ Require Import Coq.Program.Equality.
 
 Open Scope string.
 
+(* TODO: fix this proof after updating aE_Step broke it *)
 Lemma let_over_branches (v M1 M2: exp) (iV: isVal v) (B: exp):
 forall g,
 (Equiv g (eIf v (eLet M1 B) (eLet M2 B)) (eLet (eIf v M1 M2) B)).
-Proof. intros. apply aE_Trans with (M' := (eIf v (bind M1 B) (bind M2 B))).
- + apply aE_Step with (e := (eIf v (bind M1 B) (bind M2 B))).
-  - auto.
+Proof. Admitted. (*  intros. apply aE_Trans with (M' := (eIf v (bind M1 B) (bind M2 B))).
+ + apply aE_Trans with (M' := (eIf v (eLet M1 B) (bind M2 B))).
+  - apply aE_Step. 
+
+aE_Step with (e' := (eIf v (bind M1 B) (bind M2 B))).
+  - .
   - auto.
  + apply aE_Trans with (M' := (eIf v (bind (eIf v M1 M2) B) (bind (eIf v M1 M2) B))).
   - apply aE_If with (p:="eqIf"); auto.
@@ -107,8 +111,8 @@ Proof. intros. apply aE_Trans with (M' := (eIf v (bind M1 B) (bind M2 B))).
     * names. apply aE_Subst. apply aE_Symm. apply aE_If_EtaFls with (p:=free "eqIf"). auto with contexts.
   - apply aE_Trans with (M' := bind (eIf v M1 M2) B).
     * apply aE_If2.
-    * eauto.
-Qed.
+    * eauto. 
+Qed.*)
 
 
 Lemma IH_naturality_if (g: env) (K : cont) (iK: cont_is_ANF K) 
@@ -133,10 +137,12 @@ intros. eapply aE_Let; auto.
 Qed.
 
 (* As seen in the paper!*)
+(*TODO: fix after change to aE_Step)*) 
 Theorem naturality (M : exp) (iM: isConf M):
   forall (K : cont) (iK: cont_is_ANF K) (G : env), (G  ⊢ (het_compose K M) ≡ (fill_hole M K))%ECCA.
-Proof.
-  induction M using term_ind.
+Proof. Admitted.
+
+(*   induction M using term_ind.
 1-8,10-11,13-16: intros; inversion iM; rewrite het_compose_comp; auto.
   + inversion iM; subst. destruct K.
     - cbn. rewrite het_compose_hole. auto.
@@ -167,7 +173,7 @@ Proof.
       * apply Equiv_cons_shift. apply IHM2; auto.
       * apply Equiv_cons_shift. apply IHM3; auto.
     - inversion H. inversion H0.
-Qed.
+Qed.*)
 Hint Resolve naturality.
 
 Open Scope ECCA.
